bedrock2/src/Basic_bopnames.v
@@ -1,0 +1,4 @@
+Module bopname.
+  Inductive bopname := add | sub | mul | and | or | xor | sru | slu | srs | lts | ltu | eq.
+End bopname.
+Notation bopname := bopname.bopname.
