bedrock2/src/ZNamesSyntax.v
@@ -1,0 +1,11 @@
+Require Import Coq.ZArith.ZArith.
+Require Import bedrock2.Syntax.
+Require Import bedrock2.Basic_bopnames.
+
+Instance ZNames : Syntax.parameters := {|
+  Syntax.varname := Z;
+  Syntax.funname := Z;
+
+  Syntax.actname := Empty_set;
+  Syntax.bopname := bopname;
+|}.
