compiler/src/Basic32Semantics.v
@@ -1,13 +1,13 @@
 Require Import Coq.ZArith.ZArith.
 Require Import bedrock2.Syntax bedrock2.Semantics.
 Require Import bedrock2.Map.UnorderedList.
-Require Import compiler.NamesInstance.
+Require Import bedrock2.ZNamesSyntax.
 Require Import compiler.Op.
 Require Import riscv.MachineWidth32.
 Require bbv.Word.
 
 Instance Basic32Semantics: bedrock2.Semantics.parameters := {|
-  syntax := compiler.NamesInstance.Names;
+  syntax := ZNames;
   word := Word.word 32;
   interp_binop bop := eval_binop bop;
 
