compiler/src/examples/TestExprImp.v
@@ -11,7 +11,7 @@ Require Import riscv.MachineWidth32.
 Require Import compiler.util.List_Map.
 Require Import compiler.Memory.
 Require Import compiler.ExprImp.
-Require Import compiler.NamesInstance.
+Require Import bedrock2.ZNamesSyntax.
 Require Import compiler.Basic32Semantics.
 
 (*
